implement iarray vectorized write
* the structure of of the read and write are very similar and should be
  factored out
- there exist first NOT working functions for factoring out the setup
  and teadown in read and write
* small change in IArray module in order to use it_to_nat

src/lib/data/Kuiper.Vectorized.IArray.fst
@@ -26,16 +26,16 @@ let ai_add
 let iarray_pts_to_4cells
   (#et:Type0)
   (#len : erased nat) (#vw : aiview len)
-  ([@@@mkey] a : iarray et vw)
+  (a : iarray et vw)
   (#[T.exact (`1.0R)] f : perm)
-  ([@@@mkey] ai : vw.sch.ait)
+  (ai : vw.sch.ait)
   // Should probably be restricted to only the elements that are accessed?
   //  this: (#v : (ai: vw.sch.ait{0 <= vw.sch.bij.ff ai /\ vw.sch.bij.ff ai < 4} -> GTot float))
   (v : et & et & et & et)
   : slprop
   =
     Pulse.Lib.WithPure.with_pure
-      ((forall (x : natlt 4). in_image vw.step.imap.f ((it_to_nat vw ai) + x)))
+      (forall (x : natlt 4). in_image vw.step.imap.f ((it_to_nat vw ai) + x))
       (fun _ ->
         // pure (SZ.fits len) **
           iarray_pts_to_cell a #f ai               v._1 ** 
@@ -43,6 +43,93 @@ let iarray_pts_to_4cells
           iarray_pts_to_cell a #f (ai_add vw ai 2) v._3 ** 
           iarray_pts_to_cell a #f (ai_add vw ai 3) v._4)
 
+let gpu_pts_to_4slice
+  (#et:Type0)
+  (#len : nat)
+  (#vw : aiview len)
+  (a : iarray et vw)
+  (#f : perm)
+  (ai : vw.sch.ait)
+  (v : (et & et & et & et))
+  : slprop
+  =
+    pure (forall (x : natlt 4). in_image vw.step.imap.f ((it_to_nat vw ai) + x)) **
+    gpu_pts_to_slice (core a) #f
+      (it_to_nat vw ai) (it_to_nat vw ai + 4) seq![v._1; v._2; v._3; v._4]
+
+ghost
+fn iarray_4cells_pts_to_gpu_4slice
+  (#et:Type0)
+  (#len : nat)
+  (#vw : aiview len)
+  (a : iarray et vw)
+  (#f : perm)
+  (ai : vw.sch.ait)
+  (v : (et & et & et & et))
+  requires iarray_pts_to_4cells a #f ai v
+  ensures
+    (* WHY DOES THIS NOT WORK? WHAT AM I MISSING? pulling it out into its own definition works no problem *)
+      // pure (forall (x : natlt 4). in_image vw.step.imap.f ((it_to_nat vw ai) + x)) **
+      // gpu_pts_to_slice (core a) #f
+      //   (it_to_nat vw ai) (it_to_nat vw ai + 4) seq![v._1; v._2; v._3; v._4]
+    gpu_pts_to_4slice a #f ai v 
+{
+  unfold iarray_pts_to_4cells a #f ai v;
+
+  (* make index look the same for concatenation *)
+  rewrite each iarray_pts_to_cell a #f ai v._1
+  as (iarray_pts_to_cell a #f (ai_add vw ai 0) v._1);
+
+  (* get gpu_pts_to_slice *)
+  unfold iarray_pts_to_cell a #f (ai_add vw ai 0) v._1;
+  unfold iarray_pts_to_cell a #f (ai_add vw ai 1) v._2;
+  unfold iarray_pts_to_cell a #f (ai_add vw ai 2) v._3;
+  unfold iarray_pts_to_cell a #f (ai_add vw ai 3) v._4;
+
+  (* concatenate into a single slice *)
+  gpu_slice_concat (core a) #f
+    (it_to_nat vw (ai_add vw ai 0))
+    (it_to_nat vw (ai_add vw ai 1))
+    (it_to_nat vw (ai_add vw ai 1) + 1);
+  gpu_slice_concat (core a) #f
+    (it_to_nat vw (ai_add vw ai 0))
+    (it_to_nat vw (ai_add vw ai 2))
+    (it_to_nat vw (ai_add vw ai 2) + 1);
+  gpu_slice_concat (core a) #f
+    (it_to_nat vw (ai_add vw ai 0))
+    (it_to_nat vw (ai_add vw ai 3))
+    (it_to_nat vw (ai_add vw ai 3) + 1);
+
+  (* appending the values gives the goal sequence *)
+  assert pure (Seq.equal
+    seq![v._1; v._2; v._3; v._4]
+    (append (append (append seq![v._1] seq![v._2]) seq![v._3]) seq![v._4]));
+  rewrite each (append (append (append seq![v._1] seq![v._2]) seq![v._3]) seq![v._4])
+  as seq![v._1; v._2; v._3; v._4];
+
+  (* make indices look the way that they are expected in the goal *)
+  rewrite each (ai_add vw ai 0) as ai;
+  fold gpu_pts_to_4slice a #f ai v;
+  ()
+}
+
+ghost
+fn gpu_array_slice_pts_to_iarray_4cells
+  (#et:Type0)
+  (#len : nat)
+  (#vw : aiview len)
+  (a : iarray et vw)
+  (#f : perm)
+  (ai : vw.sch.ait)
+  (v : (et & et & et & et))
+  requires gpu_pts_to_slice (core a) #f
+            (it_to_nat vw ai) (it_to_nat vw ai + 4) seq![v._1; v._2; v._3; v._4]
+  requires iarray_pts_to_4cells a #f ai v
+{
+  admit();
+}
+
+// #push-options "--debug SMTFail --split_queries always"
 fn iarray_vec4_read_cells
   // (#et:Type0)
   (#len : erased nat)
@@ -58,6 +145,8 @@ fn iarray_vec4_read_cells
   ensures
     pure (e == make_float4 (reveal v)._1 (reveal v)._2 (reveal v)._3 (reveal v)._4)
 {
+  // iarray_4cells_pts_to_gpu_4slice a #f (ci_to_ai vw ci) v;
+  // unfold gpu_pts_to_4slice a #f (ci_to_ai vw ci) v;
   unfold iarray_pts_to_4cells a #f (ci_to_ai vw ci) v;
 
   (* make index look the same for concatenation *)
@@ -72,36 +161,39 @@ fn iarray_vec4_read_cells
 
   (* concatenate into a single slice *)
   gpu_slice_concat (core a) #f
-    (ai_add vw (ci_to_ai vw ci) 0 |~> vw.step.imap)
-    (ai_add vw (ci_to_ai vw ci) 1 |~> vw.step.imap)
-    ((ai_add vw (ci_to_ai vw ci) 1 |~> vw.step.imap) + 1);
+    (it_to_nat vw (ai_add vw (ci_to_ai vw ci) 0))
+    (it_to_nat vw (ai_add vw (ci_to_ai vw ci) 1))
+    (it_to_nat vw (ai_add vw (ci_to_ai vw ci) 1) + 1);
   gpu_slice_concat (core a) #f
-    (ai_add vw (ci_to_ai vw ci) 0 |~> vw.step.imap)
-    (ai_add vw (ci_to_ai vw ci) 2 |~> vw.step.imap)
-    ((ai_add vw (ci_to_ai vw ci) 2 |~> vw.step.imap) + 1);
-   gpu_slice_concat (core a) #f
-    (ai_add vw (ci_to_ai vw ci) 0 |~> vw.step.imap)
-    (ai_add vw (ci_to_ai vw ci) 3 |~> vw.step.imap)
-    ((ai_add vw (ci_to_ai vw ci) 3 |~> vw.step.imap) + 1);
+    (it_to_nat vw (ai_add vw (ci_to_ai vw ci) 0))
+    (it_to_nat vw (ai_add vw (ci_to_ai vw ci) 2))
+    (it_to_nat vw (ai_add vw (ci_to_ai vw ci) 2) + 1);
+  gpu_slice_concat (core a) #f
+    (it_to_nat vw (ai_add vw (ci_to_ai vw ci) 0))
+    (it_to_nat vw (ai_add vw (ci_to_ai vw ci) 3))
+    (it_to_nat vw (ai_add vw (ci_to_ai vw ci) 3) + 1);
 
   (* vectorized read from array *)
   cw.step.compat (ci |> cw.sch.bij.gg);
   let flat_idx = ci |~> cw.step.cimap;
+  // assert pure (it_to_nat vw (ci_to_ai vw ci) + 3 < len);
+  // This assertion isn't proven without the above :(
+  // assert pure (it_to_nat vw (ci_to_ai vw ci) + 4 <= len);
   let v' = gpu_array_read_vec4 (core a) flat_idx;
 
   (* split full slice back into multiple *)
   gpu_slice_split (core a) #f
-    (ai_add vw (ci_to_ai vw ci) 0 |~> vw.step.imap)
-    (ai_add vw (ci_to_ai vw ci) 3 |~> vw.step.imap)
-    ((ai_add vw (ci_to_ai vw ci) 3 |~> vw.step.imap) + 1);
+    (it_to_nat vw (ai_add vw (ci_to_ai vw ci) 0))
+    (it_to_nat vw (ai_add vw (ci_to_ai vw ci) 3))
+    (it_to_nat vw (ai_add vw (ci_to_ai vw ci) 3) + 1);
   gpu_slice_split (core a) #f
-    (ai_add vw (ci_to_ai vw ci) 0 |~> vw.step.imap)
-    (ai_add vw (ci_to_ai vw ci) 2 |~> vw.step.imap)
-    ((ai_add vw (ci_to_ai vw ci) 2 |~> vw.step.imap) + 1);
+    (it_to_nat vw (ai_add vw (ci_to_ai vw ci) 0))
+    (it_to_nat vw (ai_add vw (ci_to_ai vw ci) 2))
+    (it_to_nat vw (ai_add vw (ci_to_ai vw ci) 2) + 1);
   gpu_slice_split (core a) #f
-    (ai_add vw (ci_to_ai vw ci) 0 |~> vw.step.imap)
-    (ai_add vw (ci_to_ai vw ci) 1 |~> vw.step.imap)
-    ((ai_add vw (ci_to_ai vw ci) 1 |~> vw.step.imap) + 1);
+    (it_to_nat vw (ai_add vw (ci_to_ai vw ci) 0))
+    (it_to_nat vw (ai_add vw (ci_to_ai vw ci) 1))
+    (it_to_nat vw (ai_add vw (ci_to_ai vw ci) 1) + 1);
 
   (* fold back *)
   fold iarray_pts_to_cell a #f (ai_add vw (ci_to_ai vw ci) 0) (reveal v)._1;
@@ -150,18 +242,19 @@ fn iarray_vec4_write_cells
   unfold iarray_pts_to_cell a (ai_add vw (ci_to_ai vw ci) 3) v0._4;
 
   (* concatenate into a single slice *)
+  (* concatenate into a single slice *)
   gpu_slice_concat (core a)
-    (ai_add vw (ci_to_ai vw ci) 0 |~> vw.step.imap)
-    (ai_add vw (ci_to_ai vw ci) 1 |~> vw.step.imap)
-    ((ai_add vw (ci_to_ai vw ci) 1 |~> vw.step.imap) + 1);
+    (it_to_nat vw (ai_add vw (ci_to_ai vw ci) 0))
+    (it_to_nat vw (ai_add vw (ci_to_ai vw ci) 1))
+    (it_to_nat vw (ai_add vw (ci_to_ai vw ci) 1) + 1);
   gpu_slice_concat (core a)
-    (ai_add vw (ci_to_ai vw ci) 0 |~> vw.step.imap)
-    (ai_add vw (ci_to_ai vw ci) 2 |~> vw.step.imap)
-    ((ai_add vw (ci_to_ai vw ci) 2 |~> vw.step.imap) + 1);
-   gpu_slice_concat (core a)
-    (ai_add vw (ci_to_ai vw ci) 0 |~> vw.step.imap)
-    (ai_add vw (ci_to_ai vw ci) 3 |~> vw.step.imap)
-    ((ai_add vw (ci_to_ai vw ci) 3 |~> vw.step.imap) + 1);
+    (it_to_nat vw (ai_add vw (ci_to_ai vw ci) 0))
+    (it_to_nat vw (ai_add vw (ci_to_ai vw ci) 2))
+    (it_to_nat vw (ai_add vw (ci_to_ai vw ci) 2) + 1);
+  gpu_slice_concat (core a)
+    (it_to_nat vw (ai_add vw (ci_to_ai vw ci) 0))
+    (it_to_nat vw (ai_add vw (ci_to_ai vw ci) 3))
+    (it_to_nat vw (ai_add vw (ci_to_ai vw ci) 3) + 1);
 
   (* vectorized write to array *)
   cw.step.compat (ci |> cw.sch.bij.gg);
@@ -178,49 +271,41 @@ fn iarray_vec4_write_cells
      (upd_seq_vec4 (append (append (append seq![v0._1] seq![v0._2]) seq![v0._3]) seq![v0._4])
        (SZ.v flat_idx - (ai_add vw (ci_to_ai vw ci) 0 |~> vw.step.imap)) v); 
 
-  // unfold (upd_seq_vec4 (append (append (append seq![v0._1] seq![v0._2]) seq![v0._3]) seq![v0._4])
-  //       (SZ.v flat_idx - (ai_add vw (ci_to_ai vw ci) 0 |~> vw.step.imap)) v);
-  admit();
+  (* make sure the sequence is in a shape that makes it obvious how to split the slice *)
   assert pure
-    (append seq![getx v; gety v; getz v] seq![getw v] ==
+    (Seq.equal
       (upd_seq_vec4 (append (append (append seq![v0._1] seq![v0._2]) seq![v0._3]) seq![v0._4])
-        (SZ.v flat_idx - (ai_add vw (ci_to_ai vw ci) 0 |~> vw.step.imap)) v));
+        (SZ.v flat_idx - (ai_add vw (ci_to_ai vw ci) 0 |~> vw.step.imap)) v)
+      (append (append (append seq![getx v] seq![gety v]) seq![getz v]) seq![getw v]));
+  rewrite each
+    upd_seq_vec4 (append (append (append seq![v0._1] seq![v0._2]) seq![v0._3]) seq![v0._4])
+        (SZ.v flat_idx - (ai_add vw (ci_to_ai vw ci) 0 |~> vw.step.imap)) v
+  as (append (append (append seq![getx v] seq![gety v]) seq![getz v]) seq![getw v]);
 
   (* split full slice back into multiple *)
   gpu_slice_split (core a)
-    (ai_add vw (ci_to_ai vw ci) 0 |~> vw.step.imap)
-    (ai_add vw (ci_to_ai vw ci) 3 |~> vw.step.imap)
-    ((ai_add vw (ci_to_ai vw ci) 3 |~> vw.step.imap) + 1);
+    (it_to_nat vw (ai_add vw (ci_to_ai vw ci) 0))
+    (it_to_nat vw (ai_add vw (ci_to_ai vw ci) 3))
+    (it_to_nat vw (ai_add vw (ci_to_ai vw ci) 3) + 1);
   gpu_slice_split (core a)
-    (ai_add vw (ci_to_ai vw ci) 0 |~> vw.step.imap)
-    (ai_add vw (ci_to_ai vw ci) 2 |~> vw.step.imap)
-    ((ai_add vw (ci_to_ai vw ci) 2 |~> vw.step.imap) + 1);
+    (it_to_nat vw (ai_add vw (ci_to_ai vw ci) 0))
+    (it_to_nat vw (ai_add vw (ci_to_ai vw ci) 2))
+    (it_to_nat vw (ai_add vw (ci_to_ai vw ci) 2) + 1);
   gpu_slice_split (core a)
-    (ai_add vw (ci_to_ai vw ci) 0 |~> vw.step.imap)
-    (ai_add vw (ci_to_ai vw ci) 1 |~> vw.step.imap)
-    ((ai_add vw (ci_to_ai vw ci) 1 |~> vw.step.imap) + 1);
-
-  // rewrite 
-
-
-
-  // rewrite each gpu_pts_to_slice (core a) #f
-  //   (ai_add vw (ci_to_ai vw ci) 0 |~> vw.step.imap)
-  //   (ai_add vw (ci_to_ai vw ci) 1 |~> vw.step.imap) seq![(reveal v)._1]
-  // as gpu_pts_to_slice (core a) #f
-  //   (ci_to_ai vw ci |~> vw.step.imap)
-  //   ((ci_to_ai vw ci |~> vw.step.imap) + 1)  seq![(reveal v)._1];
+    (it_to_nat vw (ai_add vw (ci_to_ai vw ci) 0))
+    (it_to_nat vw (ai_add vw (ci_to_ai vw ci) 1))
+    (it_to_nat vw (ai_add vw (ci_to_ai vw ci) 1) + 1);
 
   (* fold back *)
-  fold iarray_pts_to_cell a #f (ai_add vw (ci_to_ai vw ci) 0) (reveal v)._1;
-  fold iarray_pts_to_cell a #f (ai_add vw (ci_to_ai vw ci) 1) (reveal v)._2;
-  fold iarray_pts_to_cell a #f (ai_add vw (ci_to_ai vw ci) 2) (reveal v)._3;
-  fold iarray_pts_to_cell a #f (ai_add vw (ci_to_ai vw ci) 3) (reveal v)._4;
+  fold iarray_pts_to_cell a (ai_add vw (ci_to_ai vw ci) 0) (getx v);
+  fold iarray_pts_to_cell a (ai_add vw (ci_to_ai vw ci) 1) (gety v);
+  fold iarray_pts_to_cell a (ai_add vw (ci_to_ai vw ci) 2) (getz v);
+  fold iarray_pts_to_cell a (ai_add vw (ci_to_ai vw ci) 3) (getw v);
 
   (* reverse how index looks *)
-  rewrite each iarray_pts_to_cell a #f (ai_add vw (ci_to_ai vw ci) 0) (reveal v)._1
-  as iarray_pts_to_cell a #f (ci_to_ai vw ci) (reveal v)._1;
+  rewrite each iarray_pts_to_cell a (ai_add vw (ci_to_ai vw ci) 0) (getx v)
+  as iarray_pts_to_cell a (ci_to_ai vw ci) (getx v);
 
-  fold iarray_pts_to_4cells a #f (ci_to_ai vw ci) v;
- 
+  fold iarray_pts_to_4cells a (ci_to_ai vw ci) (getx v, gety v, getz v, getw v);
+  ()
 }
